per/lsubst_hyps.v
@@ -1523,6 +1523,6 @@ Qed.
 
 (*
 *** Local Variables:
-*** coq-load-path: ("." "./close/")
+*** coq-load-path: ("." "../util/" "../terms/" "../computation/" "../cequiv/" "../close/")
 *** End:
 *)
